\documentclass{article}

\usepackage{geometry}

\usepackage{amsmath}

\usepackage{graphicx}

\title{Derivación 8 (Teórico)}

\author{Juan M. Perea, Andres Lemus}

\date{06/09/2023}

\begin{document}

\maketitle

$\Omega=[(x_0,fx(x_0)),(x_1,fx(x_1)),(x_2,fx(x_2))]$\\
Iteración 1\\
$L_0(x)=\frac{(x-x_1)(x-x_2)}{(x_0-x_1)(x_0-x_2)}=\frac{x^2-xx_2-xx_1+x_1x_2}{x^2_0-x_0x_2-x_0x_1+x_1x_2}$\\
Iteración 2\\
$L_1(x)=\frac{(x-x_0)(x-x_2))}{(x_1-x_0)(x_1-x_2)}=\frac{x^{2}-xx_0-xx_2+x_0x_2}{x_1^{2}-x_1x_2-x_1x_0+x_0x_2}$\\
Iteración 3\\
$L_2(x)=\frac{(x-x_1)(x-x_0))}{(x_2-x_0)(x_2-x_1)}=\frac{x^{2}-xx_1-xx_2+x_0x_1}{x_2^{2}-x_1x_2-x_2x_0+x_0x_1}$\\
Polinomio interpolador:\\
$P(x)=f(x_0)\frac{(x-x_1)(x-x_2)}{(x_0-x_1)(x_0-x_2)}+f(x_1)\frac{(x-x_0)(x-x_2))}{(x_1-x_0)(x_1-x_2)}+f(x_2)\frac{(x-x_1)(x-x_0))}{(x_2-x_0)(x_2-x_1)}$


\end{document}